proof for reloctablesgen is broken

x86/Reloctablesgen.v
@@ -38,75 +38,6 @@ Definition instr_reloc_offset (i:instruction) : res Z :=
   | _ => Error (msg "In reloctablesgen1: Calculation of relocation offset failed: Either there is no possible relocation location or the instruction is not supported yet by relocation")
   end.
 
-(** Calculate the starting offset of the bytes
-    that need to be relocated in an instruction *)
-Definition instr_reloc_offset_more (i:instruction) : res Z :=
-  match i with
-  | Pmov_rs _ _ => OK 2
-  | Pcall (inr _) _ => OK 1
-  | Pjmp (inr _) _ => OK 1
-  | Pleal rd a =>
-    let aofs := addrmode_reloc_offset a in
-    OK (1 + aofs)
-  | Pmovl_rm _ a =>
-    let aofs := addrmode_reloc_offset a in
-    OK (1 + aofs)
-  | Pmovl_mr a _ =>
-    let aofs := addrmode_reloc_offset a in
-    OK (1 + aofs)
-  | Pmov_rm_a _ a =>
-    let aofs := addrmode_reloc_offset a in
-    OK (1 + aofs)
-  | Pmov_mr_a a _ =>
-    let aofs := addrmode_reloc_offset a in
-      OK (1 + aofs)
-  | Pmovsd_fm_a frd a
-  | Pmovsd_fm frd a =>
-    let aofs := addrmode_reloc_offset a in
-      OK (3 + aofs)
-  | Pmovsd_mf_a a fr1
-  | Pmovsd_mf a fr1 =>
-    let aofs := addrmode_reloc_offset a in
-      OK (3 + aofs)
-  | Pmovss_fm frd a =>
-    let aofs := addrmode_reloc_offset a in
-      OK (3 + aofs)
-  | Pmovss_mf a fr1 =>
-    let aofs := addrmode_reloc_offset a in
-      OK (3 + aofs)
-  | Pfldl_m a =>
-    let aofs := addrmode_reloc_offset a in
-      OK (1 + aofs)
-  | Pfstpl_m a =>
-    let aofs := addrmode_reloc_offset a in
-      OK (1 + aofs)
-  | Pflds_m a =>
-    let aofs := addrmode_reloc_offset a in
-      OK (1 + aofs)
-  | Pfstps_m a =>
-    let aofs := addrmode_reloc_offset a in
-      OK (1 + aofs)
-  | Pmovb_mr a rs =>
-    let aofs := addrmode_reloc_offset a in
-      OK (1 + aofs)
-  | Pmovw_mr a rs =>
-    let aofs := addrmode_reloc_offset a in
-      OK (2 + aofs)
-  | Pmovzb_rm rd a =>
-    let aofs := addrmode_reloc_offset a in
-      OK (2 + aofs)
-  | Pmovzw_rm rd a =>
-    let aofs := addrmode_reloc_offset a in
-      OK (2 + aofs)
-  | Pmovsb_rm rd a =>
-    let aofs := addrmode_reloc_offset a in
-      OK (2 + aofs)
-  | Pmovsw_rm rd a =>
-    let aofs := addrmode_reloc_offset a in
-      OK (2 + aofs)         
-         
-  | _ => Error (msg "Calculation of addenddum failed: Instruction not supported yet by relocation")
-  end.
 (** Calculate the addendum of an instruction *)
 Definition instr_addendum (i:instruction) : res Z :=
   do ofs <- instr_reloc_offset i;
@@ -149,6 +80,147 @@ Definition compute_instr_disp_relocentry (sofs: Z) (i:instruction) (disp: ident*
   compute_instr_abs_relocentry sofs i (Ptrofs.unsigned addend) symb.
 
 
+
+Definition transl_instr' (sofs:Z) (i: instruction) : res (list relocentry) :=
+  match i with
+    Pallocframe _ _ _
+  | Pfreeframe _ _
+  | Pload_parent_pointer _ _ => Error (msg "Source program contains pseudo instructions")
+  | Pjmp_l _
+  | Pjcc _ _
+  | Pjcc2 _ _ _
+  | Pjmptbl _ _ => Error (msg "Source program contains jumps to labels")
+  | Pjmp (inr id) sg => 
+    do e <- compute_instr_rel_relocentry sofs i id;
+      OK [e]
+  | Pcall (inr id) sg =>
+    do e <- compute_instr_rel_relocentry sofs i id;
+      OK [e]
+  | Pmov_rs rd id => 
+    do e <- compute_instr_abs_relocentry sofs i 0 id;
+      OK [e]
+  | Pmovl_rm rd (Addrmode rb ss (inr disp)) =>
+    do e <- compute_instr_disp_relocentry sofs i disp;
+      OK [e]
+  | Pmovq_rm rd a =>
+    Error [MSG "Relocation failed: "; MSG (instr_to_string i); MSG " not supported yet"]   
+  | Pmovl_mr (Addrmode rb ss (inr disp)) rs =>
+    do e <- compute_instr_disp_relocentry sofs i disp;
+      OK [e]
+  | Pmovq_mr a rs =>
+    Error [MSG "Relocation failed: "; MSG (instr_to_string i); MSG " not supported yet"]
+  | Pmovsd_fm rd (Addrmode rb ss (inr disp)) =>
+    do e <- compute_instr_disp_relocentry sofs i disp;
+      OK [e]
+  | Pmovsd_mf (Addrmode rb ss (inr disp)) r1 =>
+    do e <- compute_instr_disp_relocentry sofs i disp;
+      OK [e]
+  | Pmovss_fm rd (Addrmode rb ss (inr disp)) =>
+    do e <- compute_instr_disp_relocentry sofs i disp;
+      OK [e]
+  | Pmovss_mf (Addrmode rb ss (inr disp)) r1 =>
+    do e <- compute_instr_disp_relocentry sofs i disp;
+      OK [e]
+  | Pfldl_m (Addrmode rb ss (inr disp)) => (**r [fld] double precision *)
+    do e <- compute_instr_disp_relocentry sofs i disp;
+      OK [e]
+  | Pfstpl_m (Addrmode rb ss (inr disp)) => (**r [fstp] double precision *)
+    do e <- compute_instr_disp_relocentry sofs i disp;
+      OK [e]
+  | Pflds_m (Addrmode rb ss (inr disp)) => (**r [fld] simple precision *)
+    do e <- compute_instr_disp_relocentry sofs i disp;
+      OK [e]
+  | Pfstps_m (Addrmode rb ss (inr disp)) => (**r [fstp] simple precision *)
+    do e <- compute_instr_disp_relocentry sofs i disp;
+      OK [e]
+  (** Moves with conversion *)
+  | Pmovb_mr (Addrmode rb ss (inr disp)) rs =>    (**r [mov] (8-bit int) *)
+    do e <- compute_instr_disp_relocentry sofs i disp;
+      OK [e]
+  | Pmovw_mr a rs =>    (**r [mov] (16-bit int) *)
+    Error [MSG "Relocation failed: "; MSG (instr_to_string i); MSG " not supported yet"]
+  | Pmovzb_rm rd (Addrmode rb ss (inr disp)) =>
+    do e <- compute_instr_disp_relocentry sofs i disp;
+      OK [e]
+  | Pmovsb_rm rd (Addrmode rb ss (inr disp)) =>
+    do e <- compute_instr_disp_relocentry sofs i disp;
+      OK [e]
+  (* Error [MSG "Relocation failed: "; MSG (instr_to_string i); MSG " not supported yet"] *)
+  | Pmovzw_rm rd a =>
+    Error [MSG "Relocation failed: "; MSG (instr_to_string i); MSG " not supported yet"]
+  | Pmovsw_rm rd a =>
+    Error [MSG "Relocation failed: "; MSG (instr_to_string i); MSG " not supported yet"]
+  (** Integer arithmetic *)
+  | Pleal rd (Addrmode rb ss (inr disp))  =>
+    do e <- compute_instr_disp_relocentry sofs i disp;
+      OK [e]
+  | Pleaq rd a =>
+    Error (msg "Relocation failed: instruction not supported yet")
+  (** Saving and restoring registers *)
+  | Pmov_rm_a rd (Addrmode rb ss (inr disp)) =>  (**r like [Pmov_rm], using [Many64] chunk *)
+    do e <- compute_instr_disp_relocentry sofs i disp;
+      OK [e]
+  | Pmov_mr_a (Addrmode rb ss (inr disp)) rs =>   (**r like [Pmov_mr], using [Many64] chunk *)
+    do e <- compute_instr_disp_relocentry sofs i disp;
+      OK [e]
+  | Pmovsd_fm_a rd a => (**r like [Pmovsd_fm], using [Many64] chunk *)
+    Error [MSG "Relocation failed:"; MSG (instr_to_string i); MSG "not supported yet"]
+  | Pmovsd_mf_a a r1 =>  (**r like [Pmovsd_mf], using [Many64] chunk *)
+    Error [MSG "Relocation failed:"; MSG (instr_to_string i); MSG "not supported yet"]
+  | _ =>
+    OK []
+  end.
+
+
+Definition ready_for_proof (i: instruction) : bool :=
+  match i with
+  | Pjmp_l_rel jofs => true
+  | Pjcc_rel c jofs => true
+  | Pcall (inr id) _ => true
+  | Pleal rd a => true
+  | Pxorl_r rd => true
+  | Paddl_ri rd n => true
+  | Psubl_ri rd n => true
+  | Psubl_rr rd r1 => true
+  | Pmovl_ri rd n => true
+  | Pmov_rr rd r1 => true
+  | Pmovl_rm rd a => true
+  | Pmovl_mr a rs => true
+  | Pmov_rm_a rd a => true
+  | Pmov_mr_a a rs => true
+  | Pmov_rs rd id => true
+  | Ptestl_rr r1 r2 => true
+  | Pret => true
+  | Pimull_rr rd r1 => true
+  | Pimull_ri rd n => true
+  | Pcmpl_rr r1 r2 => true
+  | Pcmpl_ri r1 n => true
+  | Pcltd => true
+  | Pidivl r1 => true
+  | Psall_ri rd n => true
+  | Plabel _ => true
+  | Pnop => true
+  | _ => false
+  end.
+
+Section TRANSL_INSTR.
+  Variable more_inst:bool.
+  
+  Definition transl_instr (sofs:Z) (i: instruction) : res (list relocentry) :=
+    if more_inst then
+      transl_instr' sofs i
+    else if ready_for_proof i then
+           transl_instr' sofs i
+         else
+           Error[MSG (instr_to_string i);MSG" not ready for relocation"].
+
+
+
+
+
+
+
+(* 
 Definition transl_instr (sofs:Z) (i: instruction) : res (list relocentry) :=
   match i with
     Pallocframe _ _ _
@@ -225,7 +297,7 @@ Definition transl_instr (sofs:Z) (i: instruction) : res (list relocentry) :=
     Error (msg "Relocation failed: instruction not supported yet")
   | _ =>
     OK []
-  end.
+  end. *)
 
 
 
@@ -237,6 +309,8 @@ Definition acc_instrs r i :=
 Definition transl_code (c:code) : res reloctable :=
   do (_, rtbl) <- fold_left acc_instrs c (OK (0, []));
   OK rtbl.
+
+
 
 (** ** Translation of global variables *)
 
@@ -309,18 +383,8 @@ Definition unsupported i :=
   | Pmovq_mr _ _
   | Pmovsd_fm_a _ _
   | Pmovsd_mf_a _ _
-  | Pmovsd_fm _ _
-  | Pmovsd_mf _ _
-  | Pmovss_fm _ _
-  | Pmovss_mf _ _
-  | Pfldl_m _
-  | Pfstpl_m _
-  | Pflds_m _
-  | Pfstps_m _
-  | Pmovb_mr _ _
   | Pmovw_mr _ _
-  | Pmovzb_rm _ _
-  | Pmovsb_rm _ _
+  (* | Pmovsb_rm _ _ *)
   | Pmovzw_rm _ _
   | Pmovsw_rm _ _
   | Pleaq _ _
@@ -330,38 +394,110 @@ Definition unsupported i :=
   | _ => false
   end.
 
-
-Definition id_eliminate (i:instruction):res (instruction):=
+Definition id_eliminate' (i:instruction):res (instruction):=
   if unsupported i
   then Error (msg "unsupported instruction in id_eliminate")
   else 
     match i with
-  | Pjmp (inr id) sg =>
-    OK (Pjmp (inr xH) sg)
-  | Pcall (inr id) sg =>
-    OK (Pcall (inr xH) sg)
-  | Pmov_rs rd id =>
-    OK (Pmov_rs rd xH)
-  | Pmovl_rm rd (Addrmode rb ss (inr disp)) =>
-    let '(id, ptrofs) := disp in
-    OK (Pmovl_rm rd (Addrmode rb ss (inr (xH,ptrofs))))
-  | Pmovl_mr (Addrmode rb ss (inr disp)) rs =>
-    let '(id, ptrofs) := disp in
-    OK (Pmovl_mr (Addrmode rb ss (inr (xH, ptrofs))) rs)
-  (** Integer arithmetic *)
-  | Pleal rd (Addrmode rb ss (inr disp))  =>
-    let '(id, ptrofs) := disp in
-    OK (Pleal rd (Addrmode rb ss (inr (xH, ptrofs))))
-  (** Saving and restoring registers *)
-  | Pmov_rm_a rd (Addrmode rb ss (inr disp)) =>  (**r like [Pmov_rm], using [Many64] chunk *)
-    let '(id, ptrofs) := disp in
-    OK (Pmov_rm_a rd (Addrmode rb ss (inr (xH, ptrofs))))
-  | Pmov_mr_a (Addrmode rb ss (inr disp)) rs =>   (**r like [Pmov_mr], using [Many64] chunk *)
-    let '(id, ptrofs) := disp in
-    OK (Pmov_mr_a (Addrmode rb ss (inr (xH, ptrofs))) rs)
-  | _ =>
-    OK i
+    | Pjmp (inr id) sg =>
+      OK (Pjmp (inr xH) sg)
+    | Pcall (inr id) sg =>
+      OK (Pcall (inr xH) sg)
+    | Pmov_rs rd id =>
+      OK (Pmov_rs rd xH)
+    | Pmovl_rm rd (Addrmode rb ss (inr disp)) =>
+      let '(id, ptrofs) := disp in
+      OK (Pmovl_rm rd (Addrmode rb ss (inr (xH,ptrofs))))
+    | Pmovl_mr (Addrmode rb ss (inr disp)) rs =>
+      let '(id, ptrofs) := disp in
+      OK (Pmovl_mr (Addrmode rb ss (inr (xH, ptrofs))) rs)
+    | Pfldl_m (Addrmode rb ss (inr disp)) =>
+      let '(id, ptrofs) := disp in
+      OK (Pfldl_m (Addrmode rb ss (inr (xH, ptrofs))))
+    | Pfstpl_m (Addrmode rb ss (inr disp)) =>
+      let '(id, ptrofs) := disp in
+      OK (Pfstpl_m (Addrmode rb ss (inr (xH, ptrofs))))
+    | Pflds_m (Addrmode rb ss (inr disp)) =>
+      let '(id, ptrofs) := disp in
+      OK (Pflds_m (Addrmode rb ss (inr (xH, ptrofs))))
+    | Pfstps_m (Addrmode rb ss (inr disp)) =>
+      let '(id, ptrofs) := disp in
+      OK (Pfstps_m (Addrmode rb ss (inr (xH, ptrofs))))
+    | Pmovsd_fm rd (Addrmode rb ss (inr disp)) =>
+      let '(id, ptrofs) := disp in
+      OK (Pmovsd_fm rd (Addrmode rb ss (inr (xH, ptrofs))))
+    | Pmovsd_mf (Addrmode rb ss (inr disp)) rs =>
+      let '(id, ptrofs) := disp in
+      OK (Pmovsd_mf (Addrmode rb ss (inr (xH, ptrofs))) rs)
+    | Pmovss_fm rd (Addrmode rb ss (inr disp)) =>
+      let '(id, ptrofs) := disp in
+      OK (Pmovss_fm rd (Addrmode rb ss (inr (xH, ptrofs))))
+    | Pmovss_mf (Addrmode rb ss (inr disp)) rs =>
+      let '(id, ptrofs) := disp in
+      OK (Pmovss_mf (Addrmode rb ss (inr (xH, ptrofs))) rs)       
+    (** Moves with conversion *)
+    | Pmovb_mr (Addrmode rb ss (inr disp)) rs =>
+      let '(id, ptrofs) := disp in
+      OK (Pmovb_mr (Addrmode rb ss (inr (xH, ptrofs))) rs)
+    | Pmovzb_rm rd (Addrmode rb ss (inr disp)) =>
+      let '(id, ptrofs) := disp in
+      OK (Pmovzb_rm rd (Addrmode rb ss (inr (xH, ptrofs))))
+    (** Integer arithmetic *)
+    | Pleal rd (Addrmode rb ss (inr disp))  =>
+      let '(id, ptrofs) := disp in
+      OK (Pleal rd (Addrmode rb ss (inr (xH, ptrofs))))
+    (** Saving and restoring registers *)
+    | Pmov_rm_a rd (Addrmode rb ss (inr disp)) =>  (**r like [Pmov_rm], using [Many64] chunk *)
+      let '(id, ptrofs) := disp in
+      OK (Pmov_rm_a rd (Addrmode rb ss (inr (xH, ptrofs))))
+    | Pmov_mr_a (Addrmode rb ss (inr disp)) rs =>   (**r like [Pmov_mr], using [Many64] chunk *)
+      let '(id, ptrofs) := disp in
+      OK (Pmov_mr_a (Addrmode rb ss (inr (xH, ptrofs))) rs)
+    | _ =>
+      OK i
     end.
+
+Definition id_eliminate (i:instruction):res (instruction):=
+  if more_inst then
+    id_eliminate' i
+  else if ready_for_proof i then
+         id_eliminate' i
+       else
+         Error[MSG (instr_to_string i);MSG" not ready for id_eliminate"].
+    
+
+
+(* Definition id_eliminate (i:instruction):res (instruction):= *)
+  (* if unsupported i *)
+  (* then Error (msg "unsupported instruction in id_eliminate") *)
+  (* else  *)
+  (*   match i with *)
+  (* | Pjmp (inr id) sg => *)
+  (*   OK (Pjmp (inr xH) sg) *)
+  (* | Pcall (inr id) sg => *)
+  (*   OK (Pcall (inr xH) sg) *)
+  (* | Pmov_rs rd id => *)
+  (*   OK (Pmov_rs rd xH) *)
+  (* | Pmovl_rm rd (Addrmode rb ss (inr disp)) => *)
+  (*   let '(id, ptrofs) := disp in *)
+  (*   OK (Pmovl_rm rd (Addrmode rb ss (inr (xH,ptrofs)))) *)
+  (* | Pmovl_mr (Addrmode rb ss (inr disp)) rs => *)
+  (*   let '(id, ptrofs) := disp in *)
+  (*   OK (Pmovl_mr (Addrmode rb ss (inr (xH, ptrofs))) rs) *)
+  (* (** Integer arithmetic *) *)
+  (* | Pleal rd (Addrmode rb ss (inr disp))  => *)
+  (*   let '(id, ptrofs) := disp in *)
+  (*   OK (Pleal rd (Addrmode rb ss (inr (xH, ptrofs)))) *)
+  (* (** Saving and restoring registers *) *)
+  (* | Pmov_rm_a rd (Addrmode rb ss (inr disp)) =>  (**r like [Pmov_rm], using [Many64] chunk *) *)
+  (*   let '(id, ptrofs) := disp in *)
+  (*   OK (Pmov_rm_a rd (Addrmode rb ss (inr (xH, ptrofs)))) *)
+  (* | Pmov_mr_a (Addrmode rb ss (inr disp)) rs =>   (**r like [Pmov_mr], using [Many64] chunk *) *)
+  (*   let '(id, ptrofs) := disp in *)
+  (*   OK (Pmov_mr_a (Addrmode rb ss (inr (xH, ptrofs))) rs) *)
+  (* | _ => *)
+  (*   OK i *)
+  (*   end. *)
 
 Definition acc_id_eliminate r i :=
   do r' <- r;
@@ -396,14 +532,14 @@ Definition transl_sectable' (stbl: sectable): res sectable :=
   | _ => Error (msg "Expected section table to be [text; data], got " ++ msg (print_sectable stbl))
   end.
 
-
+End TRANSL_INSTR.
 
 End WITH_SYMB_INDEX_MAP.
 
-Definition transf_program (p:program) : res program :=
+Definition transf_program(more_inst:bool) (p:program) : res program :=
   let map := gen_symb_index_map (p.(prog_symbtable)) in
-  do (codereloc, datareloc) <- transl_sectable map (prog_sectable p);
-  do sec' <- transl_sectable' (prog_sectable p);
+  do (codereloc, datareloc) <- transl_sectable map more_inst (prog_sectable p);
+  do sec' <- transl_sectable' more_inst (prog_sectable p);
   if list_norepet_dec ident_eq (List.map fst (prog_defs p))
   then
     if list_norepet_dec ident_eq (List.map symbentry_id (prog_symbtable p))
